implement sums

theories/logrel_heaplang_sessions/rules/sum.v
@@ -1,4 +1,4 @@
-From iris_examples.logrel_heaplang_sessions Require Export lty.
+From iris_examples.logrel_heaplang_sessions Require Export lty ltyping arr.
 From iris.heap_lang Require Export lifting metatheory.
 From iris.base_logic.lib Require Import invariants.
 From iris.heap_lang Require Import notation proofmode.
@@ -13,6 +13,48 @@ End types.
 Infix "+" := lty_sum : lty_scope.
 
 Section properties.
+  Context `{heapG Σ}.
+
   Global Instance lty_sum_ne : NonExpansive2 (@lty_sum Σ).
   Proof. solve_proper. Qed.
+
+  Lemma ltyped_injl Γ e A1 A2:
+    (Γ ⊨ e : A1) -∗ Γ ⊨ InjL e : A1 + A2.
+  Proof.
+    iIntros "HA" (vs) "HΓ /=".
+    wp_apply (wp_wand with "(HA [HΓ //])").
+    iIntros (v) "HA".
+    wp_pures.
+    iLeft. iExists v. auto.
+  Qed.
+
+  Lemma ltyped_injr Γ e A1 A2:
+    (Γ ⊨ e : A2) -∗ Γ ⊨ InjR e : A1 + A2.
+  Proof.
+    iIntros "HA" (vs) "HΓ /=".
+    wp_apply (wp_wand with "(HA [HΓ //])").
+    iIntros (v) "HA".
+    wp_pures.
+    iRight. iExists v. auto.
+  Qed.
+
+  Definition paircase : val :=
+    λ: "pair" "left" "right",
+    Case "pair" "left" "right".
+  Lemma ltyped_paircase Γ A1 A2 B:
+    Γ ⊨ paircase : (A1 + A2 → (A1 → B) → (A2 → B) → B)%lty.
+  Proof.
+    iIntros (vs) "HΓ /=".
+    wp_apply wp_value.
+    iIntros (p) "Hp".
+    rewrite /paircase. wp_pures.
+    iIntros (f_left) "Hleft". wp_pures.
+    iIntros (f_right) "Hright". wp_pures.
+    iDestruct "Hp" as "[Hp|Hp]".
+    - iDestruct "Hp" as (w1 ->) "Hp". wp_pures.
+      wp_apply (wp_wand with "(Hleft [Hp //])"). iIntros (v) "HB". iApply "HB".
+    - iDestruct "Hp" as (w2 ->) "Hp". wp_pures.
+      wp_apply (wp_wand with "(Hright [Hp //])"). iIntros (v) "HB". iApply "HB".
+  Qed.
+
 End properties.
